progress on proofmode and example

theories/simplang/examples/sum.v
@@ -2,7 +2,7 @@ From simuliris.simplang Require Import lang notation tactics class_instances pro
 From iris Require Import bi.bi.
 Import bi.
 From iris.proofmode Require Import tactics.
-From simuliris.simulation Require Import slsls lifting. 
+From simuliris.simulation Require Import slsls lifting.
 
 
 
@@ -25,6 +25,7 @@ Definition diverge : val := (rec: "f" "x" := "f" "x")%V.
 (* on invalid inputs, we diverge: in the source we get stuck, so any target behaviour is okay *)
 Definition case_enc : val :=
   (λ: "x" "f" "g", if: Fst "x" = #1 then
+    let: "x" := Snd "x" in
     if: Fst "x" = #1 then "f" (Snd "x")
       else if: Fst "x" = #2
         then "g" (Snd "x")
@@ -37,7 +38,7 @@ Definition case_prim : val :=
     match: "x" with
       InjL "x" => "f" "x"
     | InjR "x" => "g" "x"
-    end).
+    end)%V.
 
 (** the value relation determining which values can be passed to a function *)
 Inductive val_rel_pure : val → val → Prop :=
@@ -49,6 +50,7 @@ Inductive val_rel_pure : val → val → Prop :=
       val_rel_pure v1 v1' →
       val_rel_pure v2 v2' →
       val_rel_pure ((#0, (v1, v2))%V) ((v1', v2')%V).
+Local Hint Constructors val_rel_pure : core.
 Definition val_rel_simp v1 v2 : PROP := (⌜val_rel_pure v1 v2⌝)%I.
 
 Instance sim_sum_lang : simul_lang PROP simp_lang :=
@@ -72,19 +74,61 @@ Definition target_prog : gmap string ectx := {[ "mul2" := fun_to_ectx mul2_targe
 
 (** We want to prove: *)
 
+From iris.proofmode Require Import coq_tactics reduction.
+From iris.proofmode Require Export tactics.
+
 Lemma mul2_sim:
   ⊢ ∀ v_t v_s, val_rel v_t v_s -∗
     mul2_target (of_val v_t) ⪯ mul2_source (of_val v_s) {{λ v_t' v_s', val_rel v_t' v_s' }}.
 Proof.
+  iIntros (??) "%". rewrite /mul2_target /mul2_source.
+  sim_pures.
+  rewrite /case_enc /case_prim.
+  sim_pures.
+  (* TODO: automation for proving stuckness *)
+  inversion H; subst.
+  - iApply sim_source_stuck. iIntros (????) "_". iPureIntro.
+    split; first done. intros e' σ' H0. inversion H0; subst.
+    (*clear H0. *)
+    (*induction K. *)
+    (*+ inv_head_step. *)
+    (*+ *)
+
+    admit.
+  - sim_pures.
+    sim_pures_target.
+    inversion H0; subst.
+    { destruct l.
+      * sim_pures. iModIntro. iPureIntro. constructor.
+      * iApply sim_source_stuck. admit.
+      * iApply sim_source_stuck. admit.
+      * iApply sim_source_stuck. admit.
+      * iApply sim_source_stuck. admit.
+    }
+    all: admit.
+  - sim_pures. sim_pures_target.
+    inversion H0; subst.
+    { destruct l.
+      * sim_pures. iModIntro. iPureIntro. constructor.
+      * iApply sim_source_stuck. admit.
+      * iApply sim_source_stuck. admit.
+      * iApply sim_source_stuck. admit.
+      * iApply sim_source_stuck. admit.
+    }
+    all: admit.
+  - iApply sim_source_stuck. iIntros (????) "_". iPureIntro.
+    split; first done. intros e' σ' H2. inversion H2; subst.
+    admit.
+
 Admitted.
 
 
 (* TODO move *)
 Lemma step_Call e_t e_s (v_t v_s : val) f :
-  to_val e_t = Some v_t → to_val e_s = Some v_s → 
+  to_val e_t = Some v_t → to_val e_s = Some v_s →
   ⊢ val_rel v_t v_s -∗ Call f e_t ⪯ Call f e_s {{val_rel}}.
 Proof.
-  intros <-%of_to_val <-%of_to_val. 
+  intros <-%of_to_val <-%of_to_val.
   iIntros "H". rewrite sim_unfold. iIntros (????) "[H1 H2]". iModIntro.
   iRight; iRight. iExists f, empty_ectx, v_t, empty_ectx, v_s, σ_s. cbn. iFrame.
   iSplitL ""; first done. iSplitL "". { iPureIntro. constructor. }
@@ -98,11 +142,9 @@ Lemma client_sim (n : Z) :
   ⊢ target_client #n ⪯ source_client #n {{λ v_t v_s, val_rel v_t v_s }}.
 Proof.
   iStartProof. rewrite /target_client /source_client.
-  iApply sim_pure_steps; eauto. cbn. 
-  sim_expr_simpl. 
-  (* TODO: bind and further reduce target *)
-  (* TODO: fix handling of values. to_val (InjL ..) should go to InjLV .. ? *)
-  iApply step_Call. cbn. 
-
-Admitted.
+  sim_pures. sim_bind (inj1_enc #n) (InjL #n).
+  rewrite /inj1_enc.
+  sim_pures. sim_pures_target.
+  iApply step_Call; eauto.
+Qed.
 
