theories/simplang/proofmode.v
@@ -1,7 +1,7 @@
 From iris.proofmode Require Import coq_tactics reduction.
 From iris.proofmode Require Export tactics.
 From simuliris.simplang Require Import tactics class_instances notation.
-From simuliris.simulation Require Import slsls. 
+From simuliris.simulation Require Import slsls lifting language.
 From iris.prelude Require Import options.
 
 (*|
@@ -9,8 +9,8 @@ This is a heavily stripped-down version of HeapLang's proofmode support. To make
 |*)
 
 Section sim.
-Context {PROP : bi} {PROP_bupd : BiBUpd PROP} {PROP_affine : BiAffine PROP}. 
-Context {Λ : language} {s : simul_lang PROP Λ}.
+Context {PROP : bi} {PROP_bupd : BiBUpd PROP} {PROP_affine : BiAffine PROP}.
+Context {s : simul_lang PROP simp_lang}.
 Instance: Sim s := (sim_stutter (s := s)).
 
 Lemma tac_sim_expr_eval Δ Φ e_t e_t' e_s e_s' :
@@ -19,7 +19,52 @@ Lemma tac_sim_expr_eval Δ Φ e_t e_t' e_s e_s' :
   envs_entails Δ (e_t' ⪯ e_s' {{ Φ }}) → envs_entails Δ (e_t ⪯ e_s {{ Φ }}).
 Proof. by intros -> ->. Qed.
 
-End sim. 
+Lemma tac_sim_pure_both Δ n m e_t1 e_t2 e_s1 e_s2 K_t K_s Φ (ϕ ϕ' : Prop):
+  PureExec ϕ n (e_t1) (e_t2) →
+  PureExec ϕ' m (e_s1) (e_s2) →
+  ϕ → ϕ' →
+  n > 0 →
+  envs_entails Δ ((fill K_t e_t2) ⪯ (fill K_s e_s2) {{Φ}}) →
+  envs_entails Δ ((fill K_t e_t1) ⪯ (fill K_s e_s1) {{Φ}}).
+Proof using PROP_affine.
+  intros ? ????. rewrite envs_entails_eq.
+  (* We want [pure_exec_fill] to be available to TC search locally. *)
+  pose proof @pure_exec_ctx.
+  rewrite sim_pure_steps //.
+Qed.
+
+Lemma tac_sim_pure_target Δ n e_t e_t' e_s K_t Φ (ϕ : Prop):
+  PureExec ϕ n (e_t) (e_t') →
+  ϕ →
+  envs_entails Δ ((fill K_t e_t') ⪯ e_s {{Φ}}) →
+  envs_entails Δ ((fill K_t e_t) ⪯ e_s {{Φ}}).
+Proof using PROP_affine.
+  intros ? ?. rewrite envs_entails_eq.
+  (* We want [pure_exec_fill] to be available to TC search locally. *)
+  pose proof @pure_exec_ctx.
+  rewrite sim_pure_step_target //.
+Qed.
+
+Lemma tac_sim_value v_t v_s Φ Δ:
+  envs_entails Δ (|==> Φ v_t v_s) → envs_entails Δ (Val v_t ⪯ Val v_s {{ Φ }}).
+Proof using PROP_affine.
+  rewrite envs_entails_eq => ->. iIntros "H". iApply sim_bupd. by iApply sim_value.
+Qed.
+
+Lemma tac_sim_value_no_bupd v_t v_s Φ Δ:
+  envs_entails Δ (Φ v_t v_s) → envs_entails Δ (Val v_t ⪯ Val v_s {{ Φ }}).
+Proof using PROP_affine. rewrite envs_entails_eq => ->. by iApply sim_value. Qed.
+
+Lemma tac_sim_bind K_t K_s Δ Φ e_t f_t e_s f_s:
+  f_t = (λ e_t, fill K_t e_t) → (* as an eta expanded hypothesis so that we can `simpl` it *)
+  f_s = (λ e_s, fill K_s e_s) →
+  envs_entails Δ (e_t ⪯ e_s {{ λ v_t v_s, f_t (Val v_t) ⪯ f_s (Val v_s) {{ Φ }} }})%I →
+  envs_entails Δ (fill K_t e_t ⪯ fill K_s e_s {{ Φ }}).
+Proof using PROP_affine.
+  rewrite envs_entails_eq=> -> ->. intros H.
+  iIntros "H". iApply (sim_bind e_t e_s K_t K_s Φ). by iApply H.
+Qed.
+End sim.
 
 Tactic Notation "sim_expr_eval" tactic3(t) :=
   iStartProof;
@@ -31,4 +76,113 @@ Tactic Notation "sim_expr_eval" tactic3(t) :=
   end.
 Ltac sim_expr_simpl := sim_expr_eval simpl.
 
-(* TODO *)
+Ltac solve_vals_compare_safe :=
+  (* The first branch is for when we have [vals_compare_safe] in the context.
+     The other two branches are for when either one of the branches reduces to
+     [True] or we have it in the context. *)
+  fast_done || (left; fast_done) || (right; fast_done).
+
+
+(** Simplify the goal if it is [sim] of a value.
+  If the postcondition already allows a bupd, do not add a second one.
+  But otherwise, *do* add a bupd. This ensures that all the lemmas applied
+  here are bidirectional, so we never will make a goal unprovable. *)
+Ltac sim_value_head :=
+  lazymatch goal with
+  | |- envs_entails _ (sim (Val _) (Val _) (λ _ _, bupd _)) =>
+      eapply tac_sim_value_no_bupd
+  | |- envs_entails _ (sim (Val _) (Val _) (λ _ _, sim _ _ _)) =>
+      eapply tac_sim_value_no_bupd
+  | |- envs_entails _ (sim (Val _) (Val _) _) =>
+      eapply tac_sim_value
+  end.
+
+Ltac sim_finish :=
+  sim_expr_simpl;      (* simplify occurences of subst/fill *)
+  try sim_value_head;  (* in case we have reached a value, get rid of the WP *)
+  pm_prettify.        (* prettify λs caused by wp_value *)
+
+(** The argument [efoc] can be used to specify the construct that should be
+reduced. For example, you can write [wp_pure (EIf _ _ _)], which will search
+for an [EIf _ _ _] in the expression, and reduce it.
+
+The use of [open_constr] in this tactic is essential. It will convert all holes
+(i.e. [_]s) into evars, that later get unified when an occurences is found
+(see [unify e' efoc] in the code below). *)
+Tactic Notation "sim_pure_target" open_constr(efoc) :=
+  iStartProof;
+  lazymatch goal with
+  | |- envs_entails _ (sim ?e_t ?e_s ?Q) =>
+    let e_t := eval simpl in e_t in
+    reshape_expr e_t ltac:(fun K_t e_t' =>
+      unify e_t' efoc;
+      eapply (tac_sim_pure_target _ _ e_t' _ _ K_t _ _);
+      [ iSolveTC                       (* PureExec *)
+      | try solve_vals_compare_safe    (* The pure condition for PureExec --
+         handles trivial goals, including [vals_compare_safe] *)
+      | sim_finish                      (* new goal *)
+      ])
+    || fail "sim_pure_target: cannot find" efoc "in" e_t "or" efoc "is not a redex"
+  | _ => fail "sim_pure_target: not a 'sim'"
+  end.
+
+Ltac sim_pures_target :=
+  iStartProof;
+  first [ (* The `;[]` makes sure that no side-condition magically spawns. *)
+          progress repeat (sim_pure_target _; [])
+        | sim_finish (* In case sim_pure_target never ran, make sure we do the usual cleanup. *)
+        ].
+
+Tactic Notation "sim_pure" open_constr(efoc_t) open_constr(efoc_s) :=
+  iStartProof;
+  lazymatch goal with
+  | |- envs_entails _ (sim ?e_t ?e_s ?Q) =>
+    let e_t := eval simpl in e_t in
+    let e_s := eval simpl in e_s in
+    reshape_expr e_t ltac:(fun K_t e_t' =>
+      unify e_t' efoc_t;
+      reshape_expr e_s ltac:(fun K_s e_s' =>
+        unify e_s' efoc_s;
+        eapply (tac_sim_pure_both _ _ _ e_t' _ e_s' _ K_t K_s Q _ _);
+        [ iSolveTC                       (* PureExec *)
+        | iSolveTC                       (* PureExec *)
+        | try solve_vals_compare_safe    (* pure condition *)
+        | try solve_vals_compare_safe    (* pure condition *)
+        | lia                            (* pure n > 0 *)
+        | sim_finish                      (* new goal *)
+        ])
+      || fail "sim_pure: cannot find" efoc_s "in" e_s "or" efoc_s "is not a redex" (* TODO: fix error handling *)
+      )
+    || fail "sim_pure: cannot find" efoc_t "in" e_t "or" efoc_t "is not a redex"
+  | _ => fail "sim_pure: not a 'sim'"
+  end.
+
+Ltac sim_pures :=
+  iStartProof;
+  first [ (* The `;[]` makes sure that no side-condition magically spawns. *)
+          progress repeat (sim_pure _ _; [])
+        | sim_finish (* In case sim_pure never ran, make sure we do the usual cleanup. *)
+        ].
+
+
+Ltac sim_bind_core K_t K_s :=
+  lazymatch eval hnf in K_t with
+  | [] => lazymatch eval hnf in K_s with
+          | [] => idtac
+          | _ => eapply (tac_sim_bind K_t K_s); [simpl; reflexivity| simpl; reflexivity | ]
+          end
+  | _ => eapply (tac_sim_bind K_t K_s); [simpl; reflexivity| simpl; reflexivity | ]
+  end.
+
+Tactic Notation "sim_bind" open_constr(efoc_t) open_constr(efoc_s) :=
+  iStartProof;
+  lazymatch goal with
+  | |- envs_entails _ (sim ?e_t ?e_s ?Q) =>
+    first [ reshape_expr e_t ltac:(fun K_t e_t' => unify e_t' efoc_t;
+                                    first [ reshape_expr e_s ltac:(fun K_s e_s' => unify e_s' efoc_s; sim_bind_core K_t K_s)
+                                           (* TODO: fix error handling *)
+                                           | fail 1 "sim_bind: cannot find" efoc_s "in" e_s]
+                                  )
+          | fail 1 "sim_bind: cannot find" efoc_t "in" e_t ]
+  | _ => fail "sim_bind: not a 'sim"
+  end.
